
>[!rmk|*]- Existence, Uniqueness, and degree of minimal Polynomial
>Suppose $V$ is [[Finite-Dimensional Vector Space|Finite-Dimensional]] and $T \in \mathcal L (V)$. Then there is a unique [[Monic Polynomial]] $p \in \mathcal P( \mathbb{F})$ of smallest degree such that $p(T) = 0$. Furthermore, $\text{deg}(p) \le \text{dim}(V)$.

>[!def|*] Minimal Polynomial
>Suppose $V$ is [[Finite-Dimensional Vector Space|Finite-Dimensional]] and $T \in \mathcal L (V)$. Then the minimal polynomial of $T$ is the unique monic polynomial $p \in \mathcal P (\mathbb{F})$ of smallest degree such that $p(T) = 0$.

>[!rmk|2]- Procedure for Finding the minimal Polynomial
>To find the minimal polynomial $p$. One can pick some $v \in V$ and consider: $$c_0v + c_1 Tv + \dots + c_{\text{dim}(V)-1}T^{\text{dim}(V)-1}v = -T^{\text{dim}(V)}v$$and use a basis of $V$ to convert the equation above to a system of $\text{dim}(V)$ linear equations in $\text{dim}(V)$ unknowns $c_0, c_1, \dots ,c_{\text{dim}(V)}-1$. If the system has unique solutions, then they (as well as $c_{\text{dim}(V)} = 1$ ) are the coefficients to your polynomial. This is easier to do in matrix form and by considering the standard basis. See Example 1.

>[!exm|1]- Using the Procedure to find the minimal Polynomial
>Find the minimal Polynomial of $T \in \mathcal L (\mathbb{F}^5)$: $$T(a,b,c,d,e) = (-3e, 6e+a,b,c,d)$$To find the minimal Polynomial, for simplicity, let us transform it into a matrix. To do so, we input the standard basis $e_1, e_2, e_3, e_4, e_5$ and see what we get:
> - $e_1$: $T(1,0,0,0,0) = (0,1,0,0,0)$
> - $e_2$: $T(0,1,0,0,0) = (0,0,1,0,0)$
> - $e_3$: $T(0,0,1,0,0) = (0,0,0,1,0)$
> - $e_4$: $T(0,0,0,1,0) = (0,0,0,0,1)$
> - $e_5$: $T(0,0,0,0,1) = (-3, 6,0,0,0)$
> 
> Putting this in matrix form we get: $$\mathcal M(T) = \left[ \begin{array}{ccc} 0 & 0& 0& 0 &-3 \\ 1 &0  & 0& 0& 6\\ 0 & 1& 0&0  & 0 \\ 0 &0 &1 & 0 & 0\\0 &0 & 0&1 &0 \end{array} \right]$$Now we pick $v \in V$. Let us choose $v = (0,1,0,0,0)$. Thus we solve:
> - $Tv = T(0,1,0,0,0) = (0,0,1,0,0) = e_3$
> - $T^2v = T(Tv) = T(e_3) = (0,0,0,1,0) = e_4$
> - $T^3v = T(T^2v) = T(e_4) = (0,0,0,0,1) = e_5$
> - $T^4v = T(T^3v) = T(e_5) = (-3,6,-0,0,0) = -3e_1 + 6e_2$
> - $T^5v = T(T^4v) = T(-3e_1 + 6e_2) = -3T(e_1) + 6T(e_2) =-3e_2+ 6e_3$
> 
> Solving for $-T^5v$ is relatively easy here as some powers of $Tv$ map to $3e_2 - 6e_3$. Thus: $$-T^5v = 3e_2 -6e_3 = 3(v) -6(Tv) \implies3v -6Tv+T^5v = 0$$Hence our minimal polynomial is: $$3 - 6z+z^5$$

#### Useful Lemmas
>[!lemma|1]
>If $\lambda$ is an [[Eigenvalue]] of $T \in \mathcal L (V)$, then $\lambda^k$ is an eigenvalue of $T^k$.
>>[!claim|*]- Proof
>>`\begin{proof}` 
>>Since $\lambda$ is an eigenvalue of $T$, then: $$Tv = \lambda v \implies T^2v = \lambda Tv \implies T^2v = \lambda^2v \implies \dots$$Repeated application of $T$ with the steps above produces the desired result.
>> `\end{proof}`

>[!lemma|2]
>If $\lambda$ is an [[Eigenvalue]] of $T \in \mathcal L (V)$, then $c\lambda$ is an eigenvalue of $cT$.
>>[!claim|*]- Proof
>>`\begin{proof}` 
>>Since $\lambda$ is an eigenvalue of $T$, then: $$Tv = \lambda v \implies cTv = c\lambda v \implies (cT)v = (c \lambda) v$$Hence $c\lambda$ is an eigenvalue of $cT$.
>> `\end{proof}`

>[!lemma|3]
>Suppose $\lambda_1 \; \land \; \lambda_2$ have the same [[Eigenvector|Eigenvectors]], then $\lambda_1 + \lambda_2$ is an eigenvalue of $T_1+T_2$.
>>[!claim|*]- Proof
>>`\begin{proof}`
>>We have (assuming identical eigenvectors): $$(T_1+T_2)v = T_1 v + T_2 v = \lambda_1 v + \lambda_2 v = (\lambda_1 + \lambda_2)v$$Hence $\lambda_1+\lambda_2$ are [[Eigenvalue|Eigenvalues]] of $T_1 + T_2$ as desired.
>>  `\end{proof}`

>[!lemma|4]
>Suppose $T\ \in \mathcal L (V)$ is an [[Invertible Linear Maps|Invertible Linear Map]]. Then:
>1. $\lambda \ne 0$.
>2. $\lambda$ is an [[Eigenvalue]] of $T \iff \frac{1}{\lambda}$ is an eigenvalue of $T^{-1}$.
>
>>[!claim|*]- Proof
>>`\begin{proof}` We show both statements hold.
>>
>>**Part 1**: Suppose $\lambda$ is an eigenvalue of $T$, then: $$Tv = \lambda v \implies T^{-1}Tv = T^{-1}\lambda v \implies v =T^{-1}\lambda v$$Since $\lambda$ is an eigenvalue of $T$, then $v \ne 0$. If $v =0$, then $T$, by definition, would map $T(0) = 0$. Hence $\lambda \ne 0$.
>>
>>**Part 2**: We show $\iff$ the entire way: $$Tv = \lambda v \iff T^{-1}Tv = T^{-1}\lambda v \iff v = \lambda T^{-1} v \iff \frac{1}{\lambda}v = T^{-1} v$$Which holds as $\lambda \ne 0$ by Part $1$. Then by definition of an eigenvalue, we have that $\frac{1}{\lambda}$ is the eigenvalue of $T^{-1}$.
>>  `\end{proof}`
#### Important Theorems
>[!theorem|1] The minimal Polynomial and the Eigenvalues
>Suppose $V$ is [[Finite-Dimensional Vector Space|Finite-Dimensional]] and $T \in \mathcal L (V)$.
>1. The zeros of the minimal polynomial of $T$ are the [[Eigenvalue|Eigenvalues]] of $T$.
>2. If $V$ is a complex vector space, then the minimal polynomial of $T$ has the form: $$(z-\lambda_1)\dots(z-\lambda_m)$$where $\lambda_1, \dots \lambda_m$ is a list of all eigenvalues of $T$, possibly with repetitions.
>
>>[!claim|*]- Proof
>>`\begin{proof}`  We show both properties hold.
>>
>>**Part 1**: Let $p$ be the minimal polynomial of $T$. By definition, $p(T) = 0$. Furthermore, by the [[Fundamental Theorem of Algebra]]: $$\exists \: q: p(T)v = (T-\lambda_i I)q(T)v$$But $q(T) \ne 0$, hence:$$0 = (T- \lambda_i I)q(T)v$$Now $q \in \mathcal L (V)$ and $\exists \: v \in V: q(T)v \ne 0$ as if it was, then $q$ would be the minimal polynomial, which is not the case. Hence: $$0 = (T- \lambda_i I) v$$and we conclude $\lambda_i$ is the [[Eigenvalue]] associated with the [[Eigenvector]] $v$. To show that $\lambda_i$ is the zero of the minimal polynomial, consider Lemma 1, which tells us that $T^k v = \lambda_i^k v$. Thus: $$p(T)v = p(\lambda_i)v$$Because $p$ is the minimal polynomial of $T$, we have $p(T)v = 0$. Thus $p(\lambda_i) = 0$ as desired. Thus $p(\lambda_i)$ is a zero of $p$, as desired.
>>
>>**Part 2**: Suppose $V$ is a [[Finite-Dimensional Vector Space|Finite-Dimensional]] complex [[Vector Space]]. By the [[Existence of Eigenvalues]], $T \in \mathcal L (V)$ will have eigenvalues. Now suppose $\lambda$ is an eigenvalue of $T$, then by Part 1, $\lambda$ is the zero of the minimal polynomial $p$. By the [[Fundamental Theorem of Algebra]], we can write: $$(z- \lambda_1)\dots (z-\lambda_n)$$Producing the desired result.
>>`\end{proof}`

>[!theorem|2] Multiples of the minimal Polynomial
>Suppose $V$ is [[Finite-Dimensional Vector Space|Finite-Dimensional]], $T \in \mathcal L (V)$ and $q \in \mathcal P (\mathbb{F})$. Then: $q(T) = 0 \iff q$ is a polynomial multiple of the minimal polynomial of $T$.
>>[!claim|*]- Proof
>>`\begin{proof}` We show implication both ways. In the proof, let $p$ denote the minimal polynomial of $T$.
>>
>>$\implies$: Suppose $q(T) = 0$ By the division algorithm for polynomials, there exists polynomials $s,r \in \mathcal P (\mathbb{F})$: $$q = ps+r$$where $\text{deg}(r) < \text{deg}(p)$. We have: $$0 = q(T) = p(T)s(T) + r(T) = r(T)$$Hence for $q(T) = 0$ to be true, $r(T)$ must be $0$ and hence $q(T) = p(T)s(T)$. 
>>
>>$\impliedby$: Suppose $q$ is a polynomial multiple of $q$. Then: $$q(T) = p(T)s(T) = (0)s(T) = 0$$Where the equation holds since by definition of the minimal polynomial, $p(T) = 0$. The above equation implies $q(T) = 0$ as desired.
>> `\end{proof}`

>[!theorem|3] Operators on odd-dimensional Spaces
>Let $V$ be a [[Finite-Dimensional Vector Space|Finite-Dimensional]] [[Vector Space]] with $\text{dim}(V) = 2n+1 : n \in \mathbb{N}$. Then any operator $T \in \mathcal L (V)$ has an [[Eigenvalue]].

>[!corollary|1]
>Theorem $1$ gives a new proof of Corollary $1$ in [[Eigenvector|Eigenvectors]].
#### Exercises
>[!exercise|1]
>Suppose $V$ is [[Finite-Dimensional Vector Space|Finite-Dimensional]], $T \in \mathcal L (V)$ and $p$ is the minimal polynomial of $T$. Suppose $\alpha \in \mathbb{F}$. Show that the minimal polynomial of $\; T - \alpha I$ is the polynomial $q$ defined by $q(z) = p(z+ \alpha)$.
>>[!claim|*]- Proof
>>`\begin{proof}` 
>>Define $q(z) = p(z+ \alpha)$, we will show that it is the minimal polynomial of $T- \alpha I$. To do so, we must show two things:
>>1. Show $q(T- \alpha I) = 0$ (only shows it is a multiple of the minimal polynomial by Theorem 2).
>>2. Show $q$ is indeed the minimal polynomial.
>>
>>**Part 1**:
>>Since $q(z) = p(z+ \alpha)$, we have: $$q(T - \alpha I) = p(T - \alpha I + \alpha I) = p(T) = 0$$Hence $q$ is a multiple of the minimal polynomial. (The above equation holds as, by definition of $q$, we must add $\alpha$. Since we work with $T$, we add $\alpha I$).
>>
>>**Part 2**: 
>>Suppose $h$ is the minimal polynomial of $\: T - \alpha I$. Since $q$ is speculated to be a multiple of the minimal polynomial, we have: $$q(z) = h(z)s(z)$$Then by definition: $$q(T- \alpha I) = h(T- \alpha I) s(T - \alpha I) \implies p(T) = hs( T- \alpha I)$$Now a shifted version of the minimal polynomial should still have the same degree. Since $h$ is assumed to be the minimal polynomial, $\text{deg}(p) = \text{deg}(h)$. The only way this is possible is if $s = 1$ (thus no powers will be multiplied in). Hence: $$q(z) = h(z)(1) \implies q(z) = h(z)$$Since $h$ is the minimal polynomial, by definition of equality and by uniqueness of the minimal polynomial, we conclude $q$ is indeed the minimal polynomial of $\; T - \alpha I$ as desired.
>> `\end{proof}`

>[!exercise|2] 
>Let $V$ be a [[Finite-Dimensional Vector Space|Finite-Dimensional]] [[Vector Space]] and $T \in \mathcal L (V)$ with $c \in \mathbb{F}/\{0\}$. If $T$ has minimal polynomial $p$, then the minimal polynomial $q$ of $(cT)$ is given by: $$q(z) = c^{\text{deg}(p)}p \left( \frac{1}{c}z \right)$$
>>[!claim|*]- Proof
>>`\begin{proof}` 
>>Define $q(z) = c^{\text{deg}(p)}p \left( \frac{1}{c}z \right)$, we will show that it is the minimal polynomial of $cT$. To do so, we must show two things:
>>1. Show $q(cT) = 0$.
>>2. Show $q$ is indeed the minimal polynomial.
>>
>>**Part 1**: 
>>Since $q(z) = c^{\text{deg}(p)}p \left( \frac{1}{c}z \right)$, we have: $$q(cT) = c^{\text{deg}(p)}p \left( \frac{1}{c}cT \right) = c^{\text{deg}(p)}p(T) = c^{\text{deg}(p)}(0) = 0$$Hence $q(cT) = 0$. Thus $q(cT)$ is a multiple of the minimal polynomial.
>>
>>**Part 2**:
>>Suppose $h$ is the minimal polynomial of $cT$. Part $1$ told us that: $$q(cT) =h(cT)s(cT)$$where $s$ is some polynomial. Now notice that by definition, $\text{deg}(q) = \text{deg}(p)$. Now, let us build $h$ in such a way that it is a monic polynomial for $T$. Define: $$\frac{1}{c^{\text{deg}(p)}}h(cz) = \frac{1}{c^{\text{deg}(p)}}\left( \sum_{j=0}^{k-1}a_j(cz)^j \right) + \frac{1}{c^{\text{deg}(p)}}c^{\text{deg}(p)}z^{\text{deg}(p)}$$Which in turn produces a monic polynomial of $T$ (I simply pulled out the last term of the summation). But since $p$ is the monic polynomial of $T$, we must have, by uniqueness, that: $$p(z) = \frac{1}{c^{\text{deg}(p)}}h(cz)$$where $h(cT)$ is the minimal polynomial for $cT$. Thus now we show $q(cT) = h(cT)$ (or that $s \in \mathbb{F}$): $$q(cT) = c^{\text{deg}(p)}p \left( \frac{1}{c}cT \right)  = c^{\text{deg}(p)}p \left(T \right) = \frac{c^{\text{deg}(p)}}{c^{\text{deg}(p)}}h(cT) = h(cT)$$Since $h$ is the minimal polynomial of $cT$. Then by uniqueness, $q$ is the minimal polynomial of $cT$, as desired.
>> `\end{proof}`

>[!exercise|3]
>Let $T \in \mathcal L (\mathbb{F}^n):$ $$T(x_1, \dots x_2) = (1x_1, \dots, nx_n)$$
>1. Find the [[Eigenvalue|Eigenvalues]] and [[Eigenvector|Eigenvectors]].
>2. Find the minimal polynomial.
>
>>[!claim|*]- Solution
>>**Part 1**: By definition of eigenvalues, we want $\lambda \in \mathbb{F}$ with a non-zero associated eigenvector. (Hence $v \ne 0$). Now let $v = (x_1, \dots, x_n)$. Then: $$Tv = \lambda v \implies T(x_1, \dots, x_n) = \lambda(x_1, \dots ,x_n)$$Which gives: $$(1x_1, 2x_2, 3x_3, \dots, nx_n) =  (\lambda x_1,\lambda x_2,\lambda x_3, \dots ,\lambda x_n)$$From this, if we set $\lambda = j$ for the entry $a_j$, then all other entries $a_k : k \ne j$ will need to be $0$. In other words, the system: $$ \begin{array}{ccc} 1x_1 =\lambda x_1  \\ \vdots \\ jx_j = \lambda x_j\\ \vdots\\nx_n = \lambda x_n  \end{array}$$When given $\lambda = j$ forces $\{x_1, \dots ,x_n\}/\{x_j\} = 0$. From this, it is clear that the eigenvalues are given by $\lambda_j = j \; \; \forall \: j \in \{n : n \in \mathbb{N}\}$. (Hence $n$ **distinct** eigenvalues are present). The associated eigenvectors are given by setting $x_j = 1$ and all other components to $0$. Hence: 
>>- $\lambda = 1 \implies (1,0,0, \dots, 0)$
>>- $\lambda = 2 \implies (0,1,0, \dots, 0)$
>>- $\lambda = n \implies (0,0,0, \dots ,1)$
>>
>>**Part 2**: We know from Theorem 1 that the roots of the minimal polynomial are the eigenvalues we found. Thus: $$p(z) = (z-1 )^{m_1}\dots (z - n)^{m_n}$$Where $m_1, \dots , m_n$ are added every time we do this procedure as we usually donâ€™t know if any of the eigenvalues are repeated. However, in this case, we can clearly see that there will be no repeated eigenvalues, but let us prove it:
>>
>>Since $\text{deg}(p) \le \text{dim}(\mathbb{F}^n) = n$ (by Corollary $1$ in [[Eigenvector|Eigenvectors]]). If any $m_j > 1$, we will clearly have $\text{deg}(p) > \text{dim}(\mathbb{F}^n)$ since we already had $n$ distinct eigenvalues. Hence $m_1 = \dots = m_n$. Thus: $$p(z) = (z-1)\dots(z-n)$$Is our minimal polynomial.