Recap from previous

>[!def|*] Absolute Convergence
>A series $\sum_{k=1}^\infty a_k$ converges absolutely if $\sum_{k=1}^\infty |a_k|$ converges.

>[!def|*] Conditional Convergence
>A series converges conditionally if it does not converge absolutely.

The new stuff

>[!theorem|*] Root Test
>Let $a_k$ be a sequence $\; \land \; L = \limsup_{k \rightarrow \infty} \sqrt[k]{|a_k|}$. Then:
>- If $L > 1 \implies \sum_{k=1}^\infty a_k$ diverges
>- If $L<1 \implies \sum_{k=1}^\infty a_k$ converges
>- If $L = 1 \implies$ Nothing can be said
>
>>[!claim|*]- Proof
>>`\begin{proof}` We prove the first two cases:
>>**$L<1$ case**: If $L = limsup_{k \rightarrow \infty} \sqrt[k]{|a_k|} < 1$, then by a practice midterm problem, for any $r$ with $L < r<1$, there are finitely many $k: r< \sqrt[k]{|a_k|}$ so, $\exists \; N : \sqrt[k]{|a_k|} < r \; \; \forall k \ge N$. Then $\sum_{k=N+1}^\infty r^k$ is a geometric series and converges since $0<r<1$. 
>>Then since $\sqrt[k]{|a_k|} < r$, we have $|a_k| < r^k \; \forall k \ge N$. Thus $\sum_{k=N+1}^\infty |a_k|$ converges by the comparison test, and since $\sum_{k=0}^\infty |a_k|$ is only different at finitely many terms, it also converges.  
>>
>>**$L>1$ case**: If $L = limsup_{k \rightarrow \infty} \sqrt[k]{|a_k|} > 1$, by the practice midterm problem, $\exists \;$ an infinite number of $k : \sqrt[k]{|a_k|} > 1$. Therefore $a_k$ does not converge to $0$. 
>>Thus, by the divergence criterion, $\sum_{k=0}^\infty a_k$ diverges.
>>
>>**$L=1$ case**: If $L= 1$, we know $\sum_{k=1}^\infty \frac{1}{k}$ diverges and $limsup_{k \rightarrow \infty} \sqrt[k]{\frac{1}{k}} = 1$. Furthermore, $\sum_{k=1}^\infty \frac{1}{k^2}$ converges and $limsup_{k \rightarrow \infty} \sqrt[k]{\frac{1}{k}} = 1$. This is just showing both cases can happen.
>>  `\end{proof}`

>[!exm|*] Using the Root Test
>Consider $\sum_{k=1}^\infty (\frac{2k+3}{3k+2})^k$. We will apply the root test to get rid of the $k$ power. Thus $\sqrt[k]{|a_k|} = (\frac{2k+3}{3k+2})$. It is clear that the limit of this is $\frac{2}{3} < 1$. By the root test, the series is convergent. 

>[!exm|*] A more complicated example
>Consider: $$\sum_{k=1}^\infty a_k \; \text{where} \; a_k=\begin{cases} (\frac{1}{k})^k & k \; \text{odd}\\ (\frac{1}{2})^k & k \; \text{even} \end{cases}$$Then: $$\sqrt[n]{|a_k|} = \begin{cases} \frac{1}{k} & k \; \text{odd} \\ \frac{1}{2} & k \; \text{even} \end{cases}$$
>Clearly $limsup_{k \rightarrow \infty} \sqrt[k]{|a_k|} = \frac{1}{2} < 1$ This is convergent.

>[!exm|*] Ratio Test
>Consider $\sum_{k=1}^\infty (\frac{k^k}{k!})$. Then $$\lim_{k \rightarrow \infty} \frac{a_{k+1}}{a_k} = \lim_{k \rightarrow \infty} (1 + \frac{1}{k})^k = e > 1$$Thus our series diverges (The simplification steps were skipped).

>[!theorem|*] Cauchy Criterion for Series
>$\sum_{k=1}^\infty a_k$ converges $\iff$ $\forall \; \epsilon > 0, \; \exists \; N: | \sum_{k=1}^\infty a_k| < \epsilon$ whenever $m>n \ge N$.
>>[!claim|*]- Proof
>>`\begin{proof}` $\sum_{k=1}^\infty a_k$ converges $\iff$ $S_n$ converges.
>>Recall $S_n$ converges $\iff$ $S_n$ is Cauchy.
>>Recall $S_n$ is Cauchy $\iff$ $\forall \; \epsilon > 0, \exists \; N: |S_n - S_m = |a_{n+1} + a_{n+2} + \dots + a_m| < \epsilon$ whenever $m>n \ge N$.
>> `\end{proof}`

>[!theorem|*] Alternating Series Test
>Suppose $a_k$ is a sequence satisfying:
> - $\lim_{k \rightarrow \infty} a_k = 0$ (Required by divergence criterion)
> - $|a_k| \ge |a_{k+1}|$ $\forall \; k > K \in \mathbb{N}$
> - $\frac{a_{k+1}}{a_k} < 0 \; \forall \; k \in \mathbb{N}$ (Guarantees Alternating)
> 
> Then $\sum_{k=1}^\infty a_k$ converges.
>>[!claim|*] Proof
>>`\begin{proof}` Let $a_0 >0$ without loss of generality. Then by property $3$, $a_{2k} > 0 \; \land \; a_{2k+1} < 0$. Then $S_0 = a_0, S_1 = a_0 + a_1 < S_0$. Since $a_1 < 0$ and since $|a_1| \le |a_0|$, we have $S_1 \ge 0$â€¦
>>Define $I_0 = [0,S_0]$ which has length $L_0 = a_0$.
>> Define $I_1 = [S_1, S_0]$ with length $L_1 = -a_1 = |a_1|$.
>> Inductively, $I_n = [S_n, S_{n-1}]$ with length $L_n = |a_n|$.
>> The intervals are nested. Thus $|a_n| \rightarrow 0$ as $n \rightarrow 0$ by property $1$ of $a_n$. 
>> PROOF NOT FINISHED
>> 
>>  `\end{proof}`

